FOL/Definition.lean
@@ -5,6 +5,8 @@ import FOL.Tactics
 
 namespace FOL
 
+namespace NV
+
 open Formula
 
 
