FOL/FreeBoundFormula.lean
@@ -1,0 +1,44 @@
+import Mathlib.Util.CompileInductive
+
+
+inductive Var : Type
+  | F : String → Var
+  | B : String → Var
+  deriving Inhabited, DecidableEq
+
+open Var
+
+inductive Formula : Type
+  | pred_ : String → List Var → Formula
+  | true_ : Formula
+  | not_ : Formula → Formula
+  | imp_ : Formula → Formula → Formula
+  | forall_ : String → Formula → Formula
+  deriving Inhabited, DecidableEq
+
+compile_inductive% Formula
+
+open Formula
+
+
+def freeToBoundVar (v : String) : Var → Var
+  | F x => if x = v then B x else F x
+  | B x => B x
+
+def replaceFreeVarFun (σ : String → String) : Var → Var
+  | F x => F (σ x)
+  | B x => B x
+
+def sub (σ : String → String) : Formula → Formula
+  | pred_ X xs => pred_ X (xs.map (replaceFreeVarFun σ))
+  | true_ => true_
+  | not_ phi => not_ (sub σ phi)
+  | imp_ phi psi => imp_ (sub σ phi) (sub σ psi)
+  | forall_ x phi => forall_ x (sub σ phi)
+
+def freeToBound (v : String) : Formula → Formula
+  | pred_ X xs => pred_ X (xs.map (freeToBoundVar v))
+  | true_ => true_
+  | not_ phi => not_ (freeToBound v phi)
+  | imp_ phi psi => imp_ (freeToBound v phi) (freeToBound v psi)
+  | forall_ x phi => forall_ x (freeToBound v phi)
